adhere to preconditions

dp/6_1.dfy
@@ -14,11 +14,19 @@ module SixOne {
      * n is a[|a|-1].
      */
     function a1(a: seq<int>): seq<int>
+    decreases a
     requires |a|>=0
     {
         if |a| == 0 then [] else
         if |a| == 1 then [a[0]] else 
-        []
+        if a2([a[0]], a2(a, a[1..]))==[a[0]] then [a[0]]
+        else if a2(a, a[1..]) == a then a else a1(a[1..])
+    }
+
+    function a2(a: seq<int>, b: seq<int>): seq<int>
+    requires |a|>0 && |b|>0
+    {
+        if M.max(S.seqSum(a), S.seqSum(b)) == S.seqSum(a) then a else b
     }
 
     /**
@@ -32,7 +40,10 @@ module SixOne {
         var a := [0];
         assert a1(a) == a;
 
+        var a'', a''' := [1, 0], [0, 0];
+        assert a2(a'', a''') == a'';
+
         var a' := [1, 0];
-        assert a1(a') == a'[0];
+        assert a1(a') == [a'[0]];
     }
 }
